<?xml version="1.0" encoding="UTF-8"?>
<!--
 copyright (c) 2015, Gabriel A. Weaver, Information Trust Institute
   at the University of Illinois, Urbana-Champaign.

  This file is part of the Cyber-Physical Topology Language for
    the Power domain.

  This ontology is available under the Creative Commons 
  Attribution-ShareAlike License.  Details about this license
  are available at the following URL:

  http://creativecommons.org/licenses/by-sa/3.0/legalcode 
-->
<rdf:RDF
    xmlns:dc="http://purl.org/dc/elements/1.1/"
    xmlns:owl="http://www.w3.org/2002/07/owl#"
    xmlns:rdf="http://www.w3.org/1999/02/22-rdf-syntax-ns#"
    xmlns:rdfs="http://www.w3.org/2000/01/rdf-schema#"
    xmlns:devos="http://cptl-c.org/device/2014/07/os/">

  <owl:Ontology rdf:about="http://cptl-c.org/device/2014/07/os">
    <dc:title>A rudimentary ontology for constructs within an Operating System</dc:title>
    <dc:description>OS-level data structures to describe systems.</dc:description>
  </owl:Ontology>

  <owl:Class rdf:about="http://cptl-c.org/device/2014/07/os/Process">
    <rdfs:subClassOf rdf:resource="http://cptl-c.org/core/2014/07/core/Asset"/>
    <rdfs:label xml:lang="en">Process</rdfs:label>
    <rdfs:comment>In computing, a process is an instance of a computer
    program that is being executed.  It contains the program code and
    its current activity.  Depending on the operating system (OS), a
    process may be made up of multiple threads of execution that
    execute instructions
    concurrently. (http://en.wikipedia.org/wiki/Process (computing))</rdfs:comment>
  </owl:Class>

  <owl:Class rdf:about="http://cptl-c.org/device/2014/07/os/File">
    <rdfs:subClassOf rdf:resource="http://cptl-c.org/core/2014/07/core/Asset"/>
    <rdfs:label xml:lang="en">File</rdfs:label>
    <rdfs:comment>A computer file is a resource for storing
    information, which is available to a computer program and is
    usually based on some kind of durable storage.
    (http://en.wikipedia.org/wiki/Computer_file)</rdfs:comment>
  </owl:Class>

  <!-- Relations -->
  <owl:ObjectProperty
      rdf:about="http://cptl-c.org/device/2014/07/os/hasIPC">
    <rdfs:subClassOf rdf:resource="http://cptl-c.org/core/2014/07/core/hasLink"/>
    <rdfs:label xml:lang="en">Has Interprocess Communications</rdfs:label>
    <rdfs:comment>In computer science, inter-process communication
    (IPC) is the activity of sharing data across multiple and commonly
    specialized processes using communication protocols.
    (http://en.wikipedia.org/wiki/Inter-process_communication) </rdfs:comment>
    <rdfs:domain rdf:resource="devos:Process"/>
    <rdfs:range rdf:resource="devos:Process"/>    
  </owl:ObjectProperty>

  <owl:ObjectProperty
      rdf:about="http://cptl-c.org/device/2014/07/os/accessesFile">
    <rdfs:subClassOf rdf:resource="http://cptl-c.org/core/2014/07/core/hasLink"/>
    <rdfs:label xml:lang="en">Accesses File</rdfs:label>
    <rdfs:comment>A relation to capture file accesses by a process.</rdfs:comment>
    <rdfs:domain rdf:resource="devos:Process"/>
    <rdfs:range rdf:resource="devos:File"/>
  </owl:ObjectProperty>

  <owl:ObjectProperty
      rdf:about="http://cptl-c.org/device/2014/07/os/createsFile">
    <rdfs:subClassOf rdf:resource="http://cptl-c.org/device/2014/07/os/accessesFile"/>
    <rdfs:label xml:lang="en">Creates File</rdfs:label>
    <rdfs:comment>A process creates a file.</rdfs:comment>
  </owl:ObjectProperty>
  
  <owl:ObjectProperty
      rdf:about="http://cptl-c.org/device/2014/07/os/readsFile">
    <rdfs:subClassOf rdf:resource="http://cptl-c.org/device/2014/07/os/accessesFile"/>
    <rdfs:label xml:lang="en">Reads File</rdfs:label>
    <rdfs:comment>A process reads a file.</rdfs:comment>
  </owl:ObjectProperty>

  <owl:ObjectProperty
      rdf:about="http://cptl-c.org/device/2014/07/os/writesFile">
    <rdfs:subClassOf rdf:resource="http://cptl-c.org/device/2014/07/os/writesFile"/>
    <rdfs:label xml:lang="en">Writes File</rdfs:label>
    <rdfs:comment>A process writes a file.</rdfs:comment>
  </owl:ObjectProperty>

  <owl:ObjectProperty
      rdf:about="http://cptl-c.org/device/2014/07/os/executesFile">
    <rdfs:subClassOf rdf:resource="http://cptl-c.org/device/2014/07/os/accessesFile"/>
    <rdfs:label xml:lang="en">Executes File</rdfs:label>
    <rdfs:comment>A process executes a file.</rdfs:comment>
  </owl:ObjectProperty>

  <owl:ObjectProperty
      rdf:about="http://cptl-c.org/device/2014/07/os/opensFile">
    <rdfs:subClassOf rdf:resource="http://cptl-c.org/device/2014/07/os/accessesFile"/>
    <rdfs:label xml:lang="en">Opens File</rdfs:label>
    <rdfs:comment>A process opens a file.</rdfs:comment>
  </owl:ObjectProperty>

  <owl:ObjectProperty
      rdf:about="http://cptl-c.org/device/2014/07/os/closesFile">
    <rdfs:subClassOf rdf:resource="http://cptl-c.org/device/2014/07/os/accessesFile"/>
    <rdfs:label xml:lang="en">Closes File</rdfs:label>
    <rdfs:comment>A process closes a file.</rdfs:comment>
  </owl:ObjectProperty>
  
</rdf:RDF>
    
