<?xml version="1.0" encoding="UTF-8"?>
<!--
 copyright (c) 2015, Gabriel A. Weaver, Information Trust Institute
   at the University of Illinois, Urbana-Champaign.

  This file is part of the Cyber-Physical Topology Language for
    the Power domain.

  This ontology is available under the Creative Commons 
  Attribution-ShareAlike License.  Details about this license
  are available at the following URL:

  http://creativecommons.org/licenses/by-sa/3.0/legalcode 
 -->
<rdf:RDF 
    xmlns:cptlc="http://cptl-c.org/core/2014/07/core/"/>
    xmlns:dc="http://purl.org/dc/elements/1.1/">
    xmlns:owl="http://www.w3.org/2002/07/owl#"
    xmlns:rdf="http://www.w3.org/1999/02/22-rdf-syntax-ns#"
    xmlns:rdfs="  http://www.w3.org/2000/01/rdf-schema#">
    
    <owl:Ontology rdf:about="http://cptl-c.org/enterprise/2015/07/enterprise_network">
      <dc:title>Enterprise Network Ontology</dc:title>
      <dc:description>An ontology to describe components of an enterprise network.</dc:description>
    </owl:Ontology>

    <owl:Class rdf:about="http://cptl-c.org/enterprise/2015/07/enterprise_network/Firewall">
      <rdfs:subClassOf rdf:resource="http://cptl-c.org/core/2014/07/core/Asset"/>
      <rdfs:label xml:lang="en">Firewall</rdfs:label>
      <rdfs:comment>In computing, a firewall is a network security
      system that controls the incoming and outgoing network traffic
      based on an applied rule set. A firewall establishes a barrier
      between a trusted, secure internal network and another network
      (e.g., the Internet) that is assumed not to be secure and
      trusted. (http://en.wikipedia.org/wiki/Firewall(computing))</rdfs:comment>
    </owl:Class>

    <owl:Class rdf:about="http://cptl-c.org/enterprise/2015/07/enterprise_network/Host">
      <rdfs:subClassOf rdf:resource="http://cptl-c.org/core/2014/07/core/Asset"/>
      <rdfs:label xml:lang="en">Host</rdfs:label>
      <rdfs:comment>A network host is a computer or other device
      connected to a computer network. (http://en.wikipedia.org/wiki/Host_(network))</rdfs:comment>
    </owl:Class>

    <owl:Class rdf:about="http://cptl-c.org/enterprise/2015/07/enterprise_network/Network">
      <rdfs:subClassOf rdf:resource="http://cptl-c.org/core/2014/07/core/Asset"/>
      <rdfs:label xml:lang="en">Network</rdfs:label>
      <rdfs:comment>A computer network or data network is a
      telecommunications network which allows computers to exchange
      data. In computer networks, networked computing devices pass
      data to each other along data connections (network
      links). (http://en.wikipedia.org/wiki/Computer_network)</rdfs:comment>
    </owl:Class>

    <owl:Class rdf:about="http://cptl-c.org/enterprise/2015/07/enterprise_network/Switch">
      <rdfs:subClassOf rdf:resource="http://cptl-c.org/core/2014/07/core/Asset"/>
      <rdfs:label xml:lang="en">Switch</rdfs:label>
      <rdfs:comment>A network switch (also called switching hub,
    bridging hub, officially MAC bridge[1]) is a computer networking
    device that connects devices together on a computer network, by
    using packet switching to receive, process and forward data to the
    destination device. Unlike less advanced network hubs, a network
    switch forwards data only to one or multiple devices that need to
    receive it, rather than broadcasting the same data out of each of
    its ports. (http://en.wikipedia.org/wiki/Network_switch)</rdfs:comment>
    </owl:Class>

</rdf:RDF>



